wip rsapss: restore the structure of the generated C code

tests/rsapss-test.c
@@ -32,6 +32,7 @@ bool print_test(
   uint8_t *sgnt_expected
 ){
   uint32_t nbLen = (modBits - (uint32_t)1U) / (uint32_t)8U + (uint32_t)1U;
+  uint32_t nLen = (modBits - (uint32_t)1U) / (uint32_t)64U + (uint32_t)1U;  
   uint8_t sgnt[nbLen];
   memset(sgnt, 0U, nbLen * sizeof (sgnt[0U]));
 
@@ -39,12 +40,12 @@ bool print_test(
   uint64_t *skey = Hacl_RSAPSS_new_rsapss_load_skey(modBits, eBits, dBits, nb, eb, db);
 
 
-  Hacl_RSAPSS_rsapss_sign(Spec_Hash_Definitions_SHA2_256, modBits, eBits, dBits, skey, saltLen, salt, msgLen, msg, sgnt);
+  Hacl_RSAPSS_rsapss_sign(nLen, Spec_Hash_Definitions_SHA2_256, modBits, eBits, dBits, skey, saltLen, salt, msgLen, msg, sgnt);
   printf("RSAPSS sign Result:\n");
   bool ok = print_result(nbLen, sgnt, sgnt_expected);
 
   printf("RSAPSS verify Result:\n");
-  bool ver = Hacl_RSAPSS_rsapss_verify(Spec_Hash_Definitions_SHA2_256, modBits, eBits, pkey, saltLen, nbLen, sgnt, msgLen, msg);
+  bool ver = Hacl_RSAPSS_rsapss_verify(nLen, Spec_Hash_Definitions_SHA2_256, modBits, eBits, pkey, saltLen, nbLen, sgnt, msgLen, msg);
   if (ver) printf("Success!\n");
   ok = ok && ver;
   return ok;
