code/rsapss/Hacl.RSAPSS.fst
@@ -5,44 +5,49 @@ open Lib.IntTypes
 module S = Spec.RSAPSS
 module Hash = Spec.Agile.Hash
 
-module IR = Hacl.Impl.RSAPSS
-module IK = Hacl.Impl.RSAPSS.Keys
+module RI = Hacl.Impl.RSAPSS
+module RK = Hacl.Impl.RSAPSS.Keys
 
 module BN = Hacl.Bignum
+module BM = Hacl.Bignum.Montgomery
 module BE = Hacl.Bignum.Exponentiation
 module BD = Hacl.Bignum.Definitions
 
 #reset-options "--z3rlimit 50 --fuel 0 --ifuel 0"
 
-val rsapss_sign: IR.rsapss_sign_st U64
-let rsapss_sign a modBits eBits dBits skey sLen salt msgLen msg sgnt =
-  [@inline_let] let ke = BE.mk_runtime_exp_uint64 (BD.blocks modBits 64ul) in
-  IR.rsapss_sign ke a modBits eBits dBits skey sLen salt msgLen msg sgnt
+val rsapss_sign: len:BN.meta_len U64 -> RI.rsapss_sign_st U64 (BE.mk_runtime_exp_uint64 len).BE.mont.BM.bn.BN.len
+let rsapss_sign len a modBits eBits dBits skey sLen salt msgLen msg sgnt =
+  RI.rsapss_sign (BE.mk_runtime_exp_uint64 len) a modBits eBits dBits skey sLen salt msgLen msg sgnt
 
 
-val rsapss_verify: IR.rsapss_verify_st U64
-let rsapss_verify a modBits eBits pkey sLen k sgnt msgLen msg =
-  [@inline_let] let ke = BE.mk_runtime_exp_uint64 (BD.blocks modBits 64ul) in
-  IR.rsapss_verify ke a modBits eBits pkey sLen k sgnt msgLen msg
+val rsapss_verify: len:BN.meta_len U64 -> RI.rsapss_verify_st U64 (BE.mk_runtime_exp_uint64 len).BE.mont.BM.bn.BN.len
+let rsapss_verify len a modBits eBits pkey sLen k sgnt msgLen msg =
+  RI.rsapss_verify (BE.mk_runtime_exp_uint64 len) a modBits eBits pkey sLen k sgnt msgLen msg
 
 
-val new_rsapss_load_pkey: IK.new_rsapss_load_pkey_st U64
+val new_rsapss_load_pkey: RK.new_rsapss_load_pkey_st U64
 let new_rsapss_load_pkey r modBits eBits nb eb =
-  IK.new_rsapss_load_pkey r modBits eBits nb eb
+  RK.new_rsapss_load_pkey RK.load_pkey_u64 r modBits eBits nb eb
 
 
-val new_rsapss_load_skey: IK.new_rsapss_load_skey_st U64
+val new_rsapss_load_skey: RK.new_rsapss_load_skey_st U64
 let new_rsapss_load_skey r modBits eBits dBits nb eb db =
-  IK.new_rsapss_load_skey r modBits eBits dBits nb eb db
+  RK.new_rsapss_load_skey RK.mk_runtime_rsapss_load_keys_uint64 r modBits eBits dBits nb eb db
 
 
-val rsapss_skey_sign: IR.rsapss_skey_sign_st U64
-let rsapss_skey_sign a modBits eBits dBits nb eb db sLen salt msgLen msg sgnt =
-  [@inline_let] let ke = BE.mk_runtime_exp_uint64 (BD.blocks modBits 64ul) in
-  IR.rsapss_skey_sign #U64 ke a modBits eBits dBits nb eb db sLen salt msgLen msg sgnt
+val rsapss_skey_sign: len:BN.meta_len U64 -> RI.rsapss_skey_sign_st U64 (BE.mk_runtime_exp_uint64 len).BE.mont.BM.bn.BN.len
+let rsapss_skey_sign len a modBits eBits dBits nb eb db sLen salt msgLen msg sgnt =
+  RI.rsapss_skey_sign
+    (BE.mk_runtime_exp_uint64 len)
+     RK.mk_runtime_rsapss_load_keys_uint64
+    (RI.mk_runtime_rsapss_uint64 len)
+    a modBits eBits dBits nb eb db sLen salt msgLen msg sgnt
 
 
-val rsapss_pkey_verify: IR.rsapss_pkey_verify_st U64
-let rsapss_pkey_verify a modBits eBits nb eb sLen k sgnt msgLen msg =
-  [@inline_let] let ke = BE.mk_runtime_exp_uint64 (BD.blocks modBits 64ul) in
-  IR.rsapss_pkey_verify #U64 ke a modBits eBits nb eb sLen k sgnt msgLen msg
+val rsapss_pkey_verify: len:BN.meta_len U64 -> RI.rsapss_pkey_verify_st U64 (BE.mk_runtime_exp_uint64 len).BE.mont.BM.bn.BN.len
+let rsapss_pkey_verify len a modBits eBits nb eb sLen k sgnt msgLen msg =
+  RI.rsapss_pkey_verify
+    (BE.mk_runtime_exp_uint64 len)
+     RK.mk_runtime_rsapss_load_keys_uint64
+    (RI.mk_runtime_rsapss_uint64 len)
+     a modBits eBits nb eb sLen k sgnt msgLen msg
